have the everywhere tactic working with beta rewrite rules, now grappling with the computational properties of the strategy.

src/FP/Classes/Applicative.v
@@ -6,11 +6,14 @@ Require Import FP.Classes.Symmetric.
 Require Import FP.Classes.Transitive.
 Require Import FP.Data.Relation.
 Require Import FP.Data.Function.
+Require Import FP.Data.Function_Q.
 Require Import FP.Data.RewriteState.
+Require Import FP.Data.RewriteState_T.
 
 Import WeakSetoid.Notation.
 Import WeakEqv.Notation.
 Import Eqv.Notation.
+Import RewriteState.Notation.
 
 Class Applicative (t:WeakSetoid -> WeakSetoid) :=
   { fret :
@@ -20,48 +23,62 @@ Class Applicative (t:WeakSetoid -> WeakSetoid) :=
       forall {A B:WeakSetoid}, 
       DD (t (A ⇨ B) ⇨ (t A ⇨ t B)) 
   ; applicative_identity : 
-      forall {A:WeakSetoid}, 
-      fapply ⊛ (fret ⊛ (idQ (A:=A))) ≃ idQ
+      forall (A:WeakSetoid), 
+      fapply ⊛ (fret ⊛ (@id_Q A)) ≃ id_Q
   ; applicative_interchange :
       forall {A B:WeakSetoid} (fT:DD (t (A ⇨ B))) (x:DD A),
-      fapply ⊛ fT ⊛ (fret ⊛ x) ≃ fapply ⊛ (fret ⊛ (apply_toQ ⊛ x)) ⊛ fT
+      fapply ⊛ fT ⊛ (fret ⊛ x) ≃ fapply ⊛ (fret ⊛ (apply_to_Q ⊛ x)) ⊛ fT
   ; applicative_homomorphism : 
       forall {A B:WeakSetoid} (f:DD (A ⇨ B)) (x:DD A), 
       fapply ⊛ (fret ⊛ f) ⊛ (fret ⊛ x) ≃ fret ⊛ (f ⊛ x)
   ; applicative_composition :
       forall {A B C:WeakSetoid} (g:DD (t (B ⇨ C))) (f:DD (t (A ⇨ B))),
-      composeQ ⊛ (fapply ⊛ g) ⊛ (fapply ⊛ f) 
-      ≃ fapply ⊛ (fapply ⊛ (fapply ⊛ (fret ⊛ composeQ) ⊛ g) ⊛ f)
+      compose_Q ⊛ (fapply ⊛ g) ⊛ (fapply ⊛ f) 
+      ≃ fapply ⊛ (fapply ⊛ (fapply ⊛ (fret ⊛ compose_Q) ⊛ g) ⊛ f)
   }.
+Ltac R_Applicative_identity :=
+  match goal with
+  | [ |- RewriteState (fapply ⊛ (fret ⊛ (@id_Q ?A))) _ _ ] => ReplaceBy (applicative_identity A)
+  end.
+Ltac R_Applicative_interchange :=
+  match goal with
+  | [ |- RewriteState (fapply ⊛ ?fT ⊛ (fret ⊛ ?x)) _ _ ] => ReplaceBy (applicative_interchange fT x)
+  end.
+Ltac R_Applicative_homomorphism :=
+  match goal with
+  | [ |- RewriteState (fapply ⊛ (fret ⊛ ?f) ⊛ (fret ⊛ ?x)) _ _ ] => ReplaceBy (applicative_homomorphism f x)
+  end.
+Ltac R_Applicative_composition :=
+  match goal with
+  | [ |- RewriteState (compose_Q ⊛ (fapply ⊛ ?g) ⊛ (fapply ⊛ ?f)) _ _ ] => ReplaceBy (applicative_composition g f)
+  end.
+Ltac R_Applicative := 
+  R_Applicative_identity || R_Applicative_homomorphism || R_Applicative_composition.
 
 Section Applicative.
   Context {t:WeakSetoid -> WeakSetoid} `{! Applicative t }.
 
   Definition fapply_fmap {A B:WeakSetoid} : DD ((A ⇨ B) ⇨ t A ⇨ t B) :=
-    composeQ ⊛ fapply ⊛ fret.
+    compose_Q ⊛ fapply ⊛ fret.
 
   Local Instance Applicative_To_Functor : Functor t := { fmap := @fapply_fmap }.
   Proof.
-    - intros ; unfold fapply_fmap.
-      ReplaceBy (composeQ_elim fapply fret (idQ (A:=A))).
-      ReplaceBy (applicative_identity (A:=A)).
-      Exit ; Reflexivity.
-    - intros ; unfold fapply_fmap.
-      ReplaceBy (composeQ_elim fapply fret (composeQ ⊛ g ⊛ f)).
-      Swap.
-      PushFun ; PushArg.
-        ReplaceBy (composeQ_elim fapply fret g).
-      Pop ; Pop.
-      PushArg.
-        ReplaceBy (composeQ_elim fapply fret f).
-      Pop.
-      ReplaceBy (applicative_composition (fret ⊛ g) (fret ⊛ f)).
-      PushArg ; PushFun ; PushArg.
-        ReplaceBy (applicative_homomorphism (composeQ (A:=A)) g).
-      Pop ; Pop ; Pop.
-      PushArg.
-        ReplaceBy (applicative_homomorphism (composeQ ⊛ g) f).
-      Pop.
-      Exit ; Reflexivity.
-  Qed.
+    Local Ltac Hammer := intros ; unfold fapply_fmap ; repeat Everywhere ltac:(R_Function_beta || R_Applicative).
+    - Hammer.
+    - Hammer.
+  Defined.
 End Applicative.
+
+(*
+Eval cbv iota beta delta 
+  [functor_identity Applicative_To_Functor
+   un_RewriteState mk_RewriteState
+   rewrite_context_intro
+   rewrite_context_elim
+   rewrite_context_push_fun
+   rewrite_context_push_arg
+   rewrite_context_pop_fun
+   rewrite_context_pop_arg
+  ] 
+in functor_identity (Functor:=Applicative_To_Functor).
+*)
