src/FP/Data/RewriteState.v
@@ -1,6 +1,5 @@
 Require Import FP.Data.WeakSetoid.
 Require Import FP.Classes.WeakEqv.
-Require Import FP.Classes.Functor.
 Require Import FP.Classes.Reflexive.
 Require Import FP.Classes.Symmetric.
 Require Import FP.Classes.Transitive.
@@ -11,6 +10,9 @@ Import WeakSetoid.Notation.
 Import WeakEqv.Notation.
 Import Eqv.Notation.
 
+Create HintDb rewrite_beta.
+
+(* Also make this a definition := it's interp, constructors are just opaque things *)
 Inductive RewriteContext : WeakSetoid -> WeakSetoid -> Type :=
   | RCTop : forall {A}, RewriteContext A A
   | RCFocusFun : 
@@ -22,9 +24,6 @@ Inductive RewriteContext : WeakSetoid -> WeakSetoid -> Type :=
 Arguments RCTop {A}.
 Arguments RCFocusFun {A B C} _ _.
 Arguments RCFocusArg {A B C} _ _.
-Local Notation "κ⊤" := RCTop.
-Local Infix "◁" := RCFocusFun (at level 60, right associativity).
-Local Infix "▷" := RCFocusArg (at level 60, right associativity).
 
 Definition rewrite_context_interp {A B:WeakSetoid} (e:DD A) (k:RewriteContext A B) : DD B.
 Proof.
@@ -43,104 +42,40 @@ Proof.
   - apply IHrc ; decide_weqv.
 Defined.
 
-Inductive RewriteState 
+Definition RewriteState 
   {A B:WeakSetoid} 
-  (focus:DD A) (context:RewriteContext A B) (goal:DD B) : Type := mk_RewriteState
-  { rewrite_state_p : rewrite_context_interp focus context ≃ goal
-  }.
-Arguments mk_RewriteState {A B} focus context goal rewrite_state_p.
-Local Notation "【  f    ∈    c    ≈    g 】" := (RewriteState f c g).
-
-Definition rewrite_context_elim {A:WeakSetoid} (e:DD A) (g:DD A) (rc:RewriteState e κ⊤ g) : e ≃ g.
-Proof.
-  destruct rc ; simpl in * ; auto.
-Defined.
-
-Ltac Enter :=
-  match goal with
-  | [ |- ?x ≃ ?y ] => apply (rewrite_context_elim x y)
-  end.
-
-Definition rewrite_context_intro 
-  {A:WeakSetoid} (e:DD A) (g:DD A) (q:e ≃ g)
-  : RewriteState e κ⊤ g := mk_RewriteState e κ⊤ g q.
-
-Ltac Exit :=
-  match goal with
-  | [ |- RewriteState ?e κ⊤ ?g ] => 
-      apply (rewrite_context_intro e g)
-  end.
-
-Definition rewrite_context_push_fun
-  {A B C:WeakSetoid} 
-  (f:DD (A ⇨ B)) (x:DD A) (k:RewriteContext B C) (g:DD C) 
-  (rc:RewriteState f (k ◁ x) g)
-  : RewriteState (f ⊛ x) k g.
-Proof.
-  destruct rc ; constructor ; simpl in *.
-  Transitivity (rewrite_context_interp (apply_toQ ⊛ x ⊛ f) k) ; auto.
-  apply rewrite_context_respect_weqv ; decide_weqv.
-Defined.
-
-Ltac PushFun :=
-  try Enter ;
-  match goal with
-  | [ |- RewriteState (?f ⊛ ?x) ?k ?g ] => apply (rewrite_context_push_fun f x k g)
-  end.
-
-Definition rewrite_context_push_arg
-  {A B C:WeakSetoid} 
-  (f:DD (A ⇨ B)) (x:DD A) (k:RewriteContext B C) (g:DD C) 
-  (rc:RewriteState x (k ▷ f) g)
-  : RewriteState (f ⊛ x) k g.
-Proof.
-  destruct rc ; constructor ; simpl in *.
-  Transitivity (rewrite_context_interp (applyQ ⊛ f ⊛ x) k) ; auto.
-  apply rewrite_context_respect_weqv ; decide_weqv.
-Defined.
-
-Ltac PushArg :=
-  try Enter ;
-  match goal with
-  | [ |- RewriteState (?f ⊛ ?x) ?k ?g ] => apply (rewrite_context_push_arg f x k g)
-  end.
-
-Definition rewrite_context_pop_fun
-  {A B C:WeakSetoid}
-  (f:DD (A ⇨ B)) (x:DD A) (k:RewriteContext B C) (g:DD C)
-  (rc:RewriteState (f ⊛ x) k g)
-  : RewriteState f (k ◁ x) g.
-Proof.
-  destruct rc ; constructor ; auto.
-Qed.
-
-Definition rewrite_context_pop_arg
-  {A B C:WeakSetoid}
-  (x:DD A) (f:DD (A ⇨ B)) (k:RewriteContext B C) (g:DD C)
-  (rc:RewriteState (f ⊛ x) k g)
-  : RewriteState x (k ▷ f) g.
-Proof.
-  destruct rc ; constructor ; auto.
-Qed.
-
-Ltac Pop :=
-  match goal with
-  | [ |- RewriteState ?f (?k ◁ ?x) ?g ] => apply (rewrite_context_pop_fun f x k g)
-  | [ |- RewriteState ?x (?k ▷ ?f) ?g ] => apply (rewrite_context_pop_arg x f k g)
-  end.
-
-Ltac Escape := repeat Pop ; Exit.
-Ltac Swap := Escape ; Symmetry ; Enter.
+  (e:DD A) (k:RewriteContext A B) (g:DD B) : Type := rewrite_context_interp e k ≃ g.
+Definition mk_RewriteState 
+  {A B:WeakSetoid}
+  (e:DD A) (k:RewriteContext A B) (g:DD B) 
+  (p:rewrite_context_interp e k ≃ g)
+  : RewriteState e k g := p.
+Definition un_RewriteState 
+  {A B:WeakSetoid}
+  (e:DD A) (k:RewriteContext A B) (g:DD B) 
+  (rs:RewriteState e k g)
+  : rewrite_context_interp e k ≃ g := rs.
+Opaque RewriteState.
 
 Definition rewrite_context_replace
   {A B:WeakSetoid} 
   (e:DD A) (e':DD A) (p:e ≃ e') (k:RewriteContext A B) (g:DD B) (rc:RewriteState e' k g)
   : RewriteState e k g.
 Proof.
-  destruct rc ; constructor.
+  apply mk_RewriteState ; apply un_RewriteState in rc.
   Transitivity (rewrite_context_interp e' k) ; auto.
   apply rewrite_context_respect_weqv ; auto.
 Defined.
+
+Definition rewrite_context_elim {A:WeakSetoid} (e:DD A) (g:DD A) (rc:RewriteState e RCTop g) : e ≃ g.
+Proof.
+  apply un_RewriteState in rc ; simpl in * ; auto.
+Defined.
+
+Ltac Enter :=
+  match goal with
+  | [ |- ?x ≃ ?y ] => apply (rewrite_context_elim x y)
+  end.
 
 Ltac ReplaceBy q :=
   try Enter ;
@@ -155,3 +90,10 @@ Ltac ReplaceWith e' :=
       let q := fresh "q" in
       refine (let q := (_ : e ≈ e') in rewrite_context_replace e e' q k g _)
   end.
+
+Module Notation.
+  Notation "κ⊤" := RCTop.
+  Infix "◁" := RCFocusFun (at level 60, right associativity).
+  Infix "▷" := RCFocusArg (at level 60, right associativity).
+  Notation "【  f    ∈    c    ≃    g 】" := (RewriteState f c g).
+End Notation.
