src/FP/Data/Function_Q.v
@@ -1,0 +1,47 @@
+Require Import FP.Data.WeakSetoid.
+Require Import FP.Data.Function.
+Require Import FP.Classes.Eqv.
+Require Import FP.Data.RewriteState.
+
+Import WeakSetoid.Notation.
+Import Eqv.Notation.
+
+Definition id_Q {A:WeakSetoid} : DD (A ⇨ A) := 
+  mk_DD (A ⇨ A) id (fun _ _ => id).
+Definition id_Q_beta {A:WeakSetoid} (x:DD A) : id_Q ⊛ x ≃ x.
+Proof.
+  decide_weqv.
+Defined.
+Ltac R_id_Q_beta :=
+  match goal with
+  | [ |- RewriteState (id_Q ⊛ ?x) _ _ ] => ReplaceBy (id_Q_beta x)
+  end.
+
+Definition compose_Q {A B C:WeakSetoid} : DD ((B ⇨ C) ⇨ (A ⇨ B) ⇨ (A ⇨ C)) :=
+  mk_DD ((B ⇨ C) ⇨ (A ⇨ B) ⇨ A ⇨ C) 
+        compose
+        (fun _ _ Rff' g g' Rgg' x x' Rxx' => Rff' (g x) (g' x') (Rgg' x x' Rxx')).
+Definition compose_Q_beta 
+  {A B C:WeakSetoid} (g:DD (B ⇨ C)) (f:DD (A ⇨ B)) (x:DD A) 
+  : compose_Q ⊛ g ⊛ f ⊛ x ≃ g ⊛ (f ⊛ x).
+Proof.
+  decide_weqv.
+Defined.
+Ltac R_compose_Q_beta :=
+  match goal with
+  | [ |- RewriteState (compose_Q ⊛ ?g ⊛ ?f ⊛ ?x) _ _ ] => ReplaceBy (compose_Q_beta g f x)
+  end.
+
+Definition apply_Q {A B:WeakSetoid} : DD ((A ⇨ B) ⇨ A ⇨ B) :=
+  mk_DD ((A ⇨ B) ⇨ A ⇨ B)
+        apply
+        (fun _ _ Rfg x y Rxy => Rfg x y Rxy).
+
+Definition flip_Q {A B C:WeakSetoid} : DD ((A ⇨ B ⇨ C) ⇨ B ⇨ A ⇨ C) :=
+    mk_DD ((A ⇨ B ⇨ C) ⇨ B ⇨ A ⇨ C)
+          flip
+          (fun _ _ Rfg y y' Ryy' x x' Rxx' => Rfg x x' Rxx' y y' Ryy').
+
+Definition apply_to_Q {A B:WeakSetoid} : DD (A ⇨ (A ⇨ B) ⇨ B) := flip_Q ⊛ apply_Q.
+
+Ltac R_Function_beta := R_id_Q_beta || R_compose_Q_beta.
