src/FP/Data/RewriteState_T.v
@@ -1,0 +1,94 @@
+Require Import FP.Data.Function_Q.
+Require Import FP.Data.WeakSetoid.
+Require Import FP.Classes.Eqv.
+Require Import FP.Classes.Transitive.
+Require Import FP.Classes.Symmetric.
+Require Import FP.Classes.Reflexive.
+Require Import FP.Data.RewriteState.
+
+Import Eqv.Notation.
+Import RewriteState.Notation.
+Import WeakSetoid.Notation.
+
+Definition rewrite_context_intro 
+  {A:WeakSetoid} (e:DD A) (g:DD A) (q:e ≃ g)
+  : RewriteState e κ⊤ g := mk_RewriteState e κ⊤ g q.
+
+Ltac Exit :=
+  match goal with
+  | [ |- RewriteState ?e κ⊤ ?g ] => 
+      apply (rewrite_context_intro e g)
+  end.
+
+Definition rewrite_context_push_fun
+  {A B C:WeakSetoid} 
+  (f:DD (A ⇨ B)) (x:DD A) (k:RewriteContext B C) (g:DD C) 
+  (rc:RewriteState f (k ◁ x) g)
+  : RewriteState (f ⊛ x) k g.
+Proof.
+  apply mk_RewriteState ; apply un_RewriteState in rc ; simpl in *.
+  Transitivity (rewrite_context_interp (apply_to_Q ⊛ x ⊛ f) k) ; auto.
+  apply rewrite_context_respect_weqv ; decide_weqv.
+Defined.
+
+Ltac PushFun :=
+  try Enter ;
+  match goal with
+  | [ |- RewriteState (?f ⊛ ?x) ?k ?g ] => apply (rewrite_context_push_fun f x k g)
+  end.
+
+Definition rewrite_context_push_arg
+  {A B C:WeakSetoid} 
+  (f:DD (A ⇨ B)) (x:DD A) (k:RewriteContext B C) (g:DD C) 
+  (rc:RewriteState x (k ▷ f) g)
+  : RewriteState (f ⊛ x) k g.
+Proof.
+  apply mk_RewriteState ; apply un_RewriteState in rc ; simpl in *.
+  Transitivity (rewrite_context_interp (apply_Q ⊛ f ⊛ x) k) ; auto.
+  apply rewrite_context_respect_weqv ; decide_weqv.
+Defined.
+
+Ltac PushArg :=
+  try Enter ;
+  match goal with
+  | [ |- RewriteState (?f ⊛ ?x) ?k ?g ] => apply (rewrite_context_push_arg f x k g)
+  end.
+
+Definition rewrite_context_pop_fun
+  {A B C:WeakSetoid}
+  (f:DD (A ⇨ B)) (x:DD A) (k:RewriteContext B C) (g:DD C)
+  (rc:RewriteState (f ⊛ x) k g)
+  : RewriteState f (k ◁ x) g.
+Proof.
+  apply mk_RewriteState ; apply un_RewriteState in rc ; auto.
+Defined.
+
+Definition rewrite_context_pop_arg
+  {A B C:WeakSetoid}
+  (x:DD A) (f:DD (A ⇨ B)) (k:RewriteContext B C) (g:DD C)
+  (rc:RewriteState (f ⊛ x) k g)
+  : RewriteState x (k ▷ f) g.
+Proof.
+  apply mk_RewriteState ; apply un_RewriteState in rc ; auto.
+Defined.
+
+Ltac Pop :=
+  match goal with
+  | [ |- RewriteState ?f (?k ◁ ?x) ?g ] => apply (rewrite_context_pop_fun f x k g)
+  | [ |- RewriteState ?x (?k ▷ ?f) ?g ] => apply (rewrite_context_pop_arg x f k g)
+  end.
+
+Ltac Escape := repeat Pop ; Exit.
+Ltac Swap := Escape ; Symmetry ; Enter.
+
+Ltac Everywhere_1 t :=
+  try Enter ;
+  match goal with
+  | [ |- RewriteState (_ ⊛ _) _ _ ] =>
+      PushFun ; Everywhere_1 t ; Pop ; PushArg ; Everywhere_1 t ; Pop ; repeat t
+  | _ => repeat t
+  end ;
+  try Exit ;
+  try Reflexivity.
+
+Ltac Everywhere t := Everywhere_1 t ; Symmetry ; Everywhere_1 t ; Symmetry.
